spec: error handling

src/lowparse/LowParse.Spec.Array.fst
@@ -20,34 +20,48 @@ let array_pred (#t: Type) (n: nat) (s: list t) : GTot Type0 =
 let fldata_array_precond
   (#k: parser_kind)
   (#t: Type0)
-  (p: parser k t)
+  (#err: Type0)
+  (p: parser k t err)
   (array_byte_size: nat)
   (elem_count: nat)
 : GTot bool
 = serialize_list_precond k &&
   k.parser_kind_high = Some k.parser_kind_low &&
+  k.parser_kind_low > 0 &&
   elem_count * k.parser_kind_low = array_byte_size
+
+let parse_list_precond_of_fldata_array_precond
+  (#k: parser_kind)
+  (#t: Type0)
+  (#err: Type0)
+  (p: parser k t err)
+  (array_byte_size: nat)
+  (elem_count: nat)
+: Pure (u: unit { k.parser_kind_low > 0 } )
+  (requires (fldata_array_precond p array_byte_size elem_count == true))
+  (ensures (fun _ -> True))
+= ()
 
 let fldata_to_array_correct
   (#k: parser_kind)
   (#t: Type0)
-  (#p: parser k t)
+  (#err: Type0)
+  (#p: parser k t err)
   (s: serializer p)
   (array_byte_size: nat)
   (elem_count: nat)
   (x: list t)
+  (u1: unit { fldata_array_precond p array_byte_size elem_count == true } )
+  (u2: unit { parse_fldata_strong_pred (serialize_list _ (parse_list_precond_of_fldata_array_precond p array_byte_size elem_count) s) array_byte_size x } )
 : Lemma
-  (requires (
-    fldata_array_precond p array_byte_size elem_count == true /\
-    parse_fldata_strong_pred (serialize_list _ s) array_byte_size x
-  ))
   (ensures (
     array_pred elem_count x
   ))
-= let y = serialize (serialize_list _ s) x in
-  assert (parse (parse_list p) y == Some (x, array_byte_size));
+= let u = (parse_list_precond_of_fldata_array_precond p array_byte_size elem_count) in
+  let y = serialize (serialize_list _ u s) x in
+  assert (parse (parse_list p u) y == Correct (x, array_byte_size));
   assert (Seq.length y == array_byte_size);
-  list_length_constant_size_parser_correct p y;
+  list_length_constant_size_parser_correct p u y;
   M.mul_reg_r elem_count (L.length x) k.parser_kind_low
 
 inline_for_extraction
@@ -57,25 +71,27 @@ inline_for_extraction
 let fldata_to_array
   (#k: parser_kind)
   (#t: Type0)
-  (#p: parser k t)
+  (#err: Type0)
+  (#p: parser k t err)
   (s: serializer p)
   (array_byte_size: nat)
   (elem_count: nat)
   (u: unit {
     fldata_array_precond p array_byte_size elem_count == true
   })
-  (x: parse_fldata_strong_t (serialize_list _ s) array_byte_size)
+  (x: parse_fldata_strong_t (serialize_list _ () s) array_byte_size)
 : Tot (array t elem_count)
 = [@inline_let]
   let (x' : list t) = x in
   [@inline_let]
-  let _ = fldata_to_array_correct s array_byte_size elem_count x' in
+  let _ = fldata_to_array_correct s array_byte_size elem_count x' () () in
   x'
 
 let fldata_to_array_inj
   (#k: parser_kind)
   (#t: Type0)
-  (#p: parser k t)
+  (#err: Type0)
+  (#p: parser k t err)
   (s: serializer p)
   (array_byte_size: nat)
   (elem_count: nat)
@@ -83,7 +99,7 @@ let fldata_to_array_inj
     fldata_array_precond p array_byte_size elem_count == true
   })
 : Lemma
-  (forall (x1 x2: parse_fldata_strong_t (serialize_list _ s) array_byte_size) .
+  (forall (x1 x2: parse_fldata_strong_t (serialize_list _ () s) array_byte_size) .
     fldata_to_array s array_byte_size elem_count u x1 == 
     fldata_to_array s array_byte_size elem_count u x2 ==>
     x1 == x2)
@@ -92,43 +108,45 @@ let fldata_to_array_inj
 let parse_array
   (#k: parser_kind)
   (#t: Type0)
-  (#p: parser k t)
+  (#err: Type0)
+  (#p: parser k t err)
   (s: serializer p)
   (array_byte_size: nat)
   (elem_count: nat)
-: Pure (parser (parse_fldata_kind array_byte_size) (array t elem_count))
+  (e: err)
+: Pure (parser (parse_fldata_kind array_byte_size) (array t elem_count) err)
   (requires (
     fldata_array_precond p array_byte_size elem_count == true
   ))
   (ensures (fun _ -> True))
 = let (u : unit { fldata_array_precond p array_byte_size elem_count == true } ) = () in
   fldata_to_array_inj s array_byte_size elem_count u;
-  parse_fldata_strong (serialize_list _ s) array_byte_size `parse_synth` (fldata_to_array s array_byte_size elem_count u)
+  parse_fldata_strong (serialize_list _ () s) array_byte_size e `parse_synth` (fldata_to_array s array_byte_size elem_count u)
 
 let array_to_fldata_correct
   (#k: parser_kind)
   (#t: Type0)
-  (#p: parser k t)
+  (#err: Type0)
+  (#p: parser k t err)
   (s: serializer p)
   (array_byte_size: nat)
   (elem_count: nat)
   (x: list t)
+  (u1: unit { fldata_array_precond p array_byte_size elem_count == true } )
+  (u2: unit { array_pred elem_count x } )
 : Lemma
-  (requires (
-    fldata_array_precond p array_byte_size elem_count == true /\
-    array_pred elem_count x
-  ))
   (ensures (
-    parse_fldata_strong_pred (serialize_list _ s) array_byte_size x
+    parse_fldata_strong_pred (serialize_list _ () s) array_byte_size x
   ))
-= let y = serialize (serialize_list _ s) x in
-  list_length_constant_size_parser_correct p y
+= let y = serialize (serialize_list _ () s) x in
+  list_length_constant_size_parser_correct p () y
 
 inline_for_extraction
 let array_to_fldata
   (#k: parser_kind)
   (#t: Type0)
-  (#p: parser k t)
+  (#err: Type0)
+  (#p: parser k t err)
   (s: serializer p)
   (array_byte_size: nat)
   (elem_count: nat)
@@ -136,17 +154,18 @@ let array_to_fldata
     fldata_array_precond p array_byte_size elem_count == true
   })
   (x: array t elem_count)
-: Tot (parse_fldata_strong_t (serialize_list _ s) array_byte_size)
+: Tot (parse_fldata_strong_t (serialize_list _ () s) array_byte_size)
 = [@inline_let]
   let (x' : list t) = x in
   [@inline_let]
-  let _ = array_to_fldata_correct s array_byte_size elem_count x' in
+  let _ = array_to_fldata_correct s array_byte_size elem_count x' () () in
   x'
 
 let array_to_fldata_to_array
   (#k: parser_kind)
   (#t: Type0)
-  (#p: parser k t)
+  (#err: Type0)
+  (#p: parser k t err)
   (s: serializer p)
   (array_byte_size: nat)
   (elem_count: nat)
@@ -161,20 +180,22 @@ let array_to_fldata_to_array
 let serialize_array
   (#k: parser_kind)
   (#t: Type0)
-  (#p: parser k t)
+  (#err: Type0)
+  (#p: parser k t err)
   (s: serializer p)
   (array_byte_size: nat)
   (elem_count: nat)
+  (e: err)
   (u: unit {
     fldata_array_precond p array_byte_size elem_count == true
   })
-: Tot (serializer (parse_array s array_byte_size elem_count))
+: Tot (serializer (parse_array s array_byte_size elem_count e))
 = fldata_to_array_inj s array_byte_size elem_count u;
   array_to_fldata_to_array s array_byte_size elem_count u u;
   serialize_synth
     _
     (fldata_to_array s array_byte_size elem_count u)
-    (serialize_fldata_strong (serialize_list _ s) array_byte_size)
+    (serialize_fldata_strong (serialize_list _ () s) array_byte_size e)
     (array_to_fldata s array_byte_size elem_count u)
     ()
 
@@ -188,12 +209,14 @@ let vldata_vlarray_precond
   (array_byte_size_max: nat)
   (#k: parser_kind)
   (#t: Type0)
-  (p: parser k t)
+  (#err: Type0)
+  (p: parser k t err)
   (elem_count_min: nat)
   (elem_count_max: nat)
 : GTot bool
 = (* constant-size serializable parser for elements *)
      serialize_list_precond k &&
+     k.parser_kind_low > 0 &&
      k.parser_kind_high = Some k.parser_kind_low &&
   (* vldata *)
      array_byte_size_min <= array_byte_size_max &&
@@ -214,23 +237,22 @@ let vldata_to_vlarray_correct
   (array_byte_size_max: nat)
   (#k: parser_kind)
   (#t: Type0)
-  (#p: parser k t)
+  (#err: Type0)
+  (#p: parser k t err)
   (s: serializer p)
   (elem_count_min: nat)
   (elem_count_max: nat)
   (x: list t)
+  (u1: unit { vldata_vlarray_precond array_byte_size_min array_byte_size_max p elem_count_min elem_count_max == true } )
+  (u2: unit { parse_bounded_vldata_strong_pred array_byte_size_min array_byte_size_max (serialize_list _ () s) x } )
 : Lemma
-  (requires (
-    vldata_vlarray_precond array_byte_size_min array_byte_size_max p elem_count_min elem_count_max == true /\
-    parse_bounded_vldata_strong_pred array_byte_size_min array_byte_size_max (serialize_list _ s) x
-  ))
   (ensures (
     vlarray_pred elem_count_min elem_count_max x
   ))
-= let y = serialize (serialize_list _ s) x in
+= let y = serialize (serialize_list _ () s) x in
   let l = L.length x in
-  assert (parse (parse_list p) y == Some (x, Seq.length y));
-  list_length_constant_size_parser_correct p y;
+  assert (parse (parse_list p ()) y == Correct (x, Seq.length y));
+  list_length_constant_size_parser_correct p () y;
   M.lt_mul_add_reg_r elem_count_min l k.parser_kind_low;
   M.lt_mul_add_reg_r l elem_count_max k.parser_kind_low
 
@@ -244,19 +266,20 @@ let vldata_to_vlarray
   (array_byte_size_max: nat)
   (#k: parser_kind)
   (#t: Type0)
-  (#p: parser k t)
+  (#err: Type0)
+  (#p: parser k t err)
   (s: serializer p)
   (elem_count_min: nat)
   (elem_count_max: nat)
   (u: unit {
     vldata_vlarray_precond array_byte_size_min array_byte_size_max p elem_count_min elem_count_max == true  
   })
-  (x: parse_bounded_vldata_strong_t array_byte_size_min array_byte_size_max (serialize_list _ s))
+  (x: parse_bounded_vldata_strong_t array_byte_size_min array_byte_size_max (serialize_list _ () s))
 : Tot (vlarray t elem_count_min elem_count_max)
 = [@inline_let]
   let x' : list t = x in
   [@inline_let]
-  let _ = vldata_to_vlarray_correct array_byte_size_min array_byte_size_max s elem_count_min elem_count_max x' in
+  let _ = vldata_to_vlarray_correct array_byte_size_min array_byte_size_max s elem_count_min elem_count_max x' () () in
   x'
 
 let vldata_to_vlarray_inj
@@ -264,7 +287,8 @@ let vldata_to_vlarray_inj
   (array_byte_size_max: nat)
   (#k: parser_kind)
   (#t: Type0)
-  (#p: parser k t)
+  (#err: Type0)
+  (#p: parser k t err)
   (s: serializer p)
   (elem_count_min: nat)
   (elem_count_max: nat)
@@ -272,7 +296,7 @@ let vldata_to_vlarray_inj
     vldata_vlarray_precond array_byte_size_min array_byte_size_max p elem_count_min elem_count_max == true  
   })
 : Lemma
-  (forall (x1 x2: parse_bounded_vldata_strong_t array_byte_size_min array_byte_size_max (serialize_list _ s)) .
+  (forall (x1 x2: parse_bounded_vldata_strong_t array_byte_size_min array_byte_size_max (serialize_list _ () s)) .
     vldata_to_vlarray array_byte_size_min array_byte_size_max s elem_count_min elem_count_max u x1 ==
     vldata_to_vlarray array_byte_size_min array_byte_size_max s elem_count_min elem_count_max u x2 ==>
     x1 == x2)
@@ -283,16 +307,19 @@ let parse_vlarray
   (array_byte_size_max: nat)
   (#k: parser_kind)
   (#t: Type0)
-  (#p: parser k t)
+  (#err: Type0)
+  (#p: parser k t err)
   (s: serializer p)
   (elem_count_min: nat)
   (elem_count_max: nat)
   (u: unit {
     vldata_vlarray_precond array_byte_size_min array_byte_size_max p elem_count_min elem_count_max == true  
   })
-: Tot (parser (parse_bounded_vldata_kind array_byte_size_min array_byte_size_max) (vlarray t elem_count_min elem_count_max))
+  (e_size_incomplete e_size_invalid e_payload: err)
+: Tot (parser (parse_bounded_vldata_kind array_byte_size_min array_byte_size_max) (vlarray t elem_count_min elem_count_max) err)
 = vldata_to_vlarray_inj array_byte_size_min array_byte_size_max s elem_count_min elem_count_max u;
-  parse_bounded_vldata_strong array_byte_size_min array_byte_size_max (serialize_list _ s)
+  parse_bounded_vldata_strong array_byte_size_min array_byte_size_max (serialize_list _ () s)
+   e_size_incomplete e_size_invalid e_payload
   `parse_synth`
   vldata_to_vlarray array_byte_size_min array_byte_size_max s elem_count_min elem_count_max u
 
@@ -301,23 +328,22 @@ let vlarray_to_vldata_correct
   (array_byte_size_max: nat)
   (#k: parser_kind)
   (#t: Type0)
-  (#p: parser k t)
+  (#err: Type0)
+  (#p: parser k t err)
   (s: serializer p)
   (elem_count_min: nat)
   (elem_count_max: nat)
   (x: list t)
+  (u1: unit { vldata_vlarray_precond array_byte_size_min array_byte_size_max p elem_count_min elem_count_max == true } )
+  (u2: unit { vlarray_pred elem_count_min elem_count_max x } )
 : Lemma
-  (requires (
-    vldata_vlarray_precond array_byte_size_min array_byte_size_max p elem_count_min elem_count_max == true /\
-    vlarray_pred elem_count_min elem_count_max x
-  ))
   (ensures (
-    parse_bounded_vldata_strong_pred array_byte_size_min array_byte_size_max (serialize_list _ s) x
+    parse_bounded_vldata_strong_pred array_byte_size_min array_byte_size_max (serialize_list _ () s) x
   ))
-= let y = serialize (serialize_list _ s) x in
+= let y = serialize (serialize_list _ () s) x in
   let l = L.length x in
-  assert (parse (parse_list p) y == Some (x, Seq.length y));
-  list_length_constant_size_parser_correct p y;
+  assert (parse (parse_list p ()) y == Correct (x, Seq.length y));
+  list_length_constant_size_parser_correct p () y;
   M.lemma_mult_le_right k.parser_kind_low elem_count_min l;
   M.lemma_mult_le_right k.parser_kind_low l elem_count_max
 
@@ -327,7 +353,8 @@ let vlarray_to_vldata
   (array_byte_size_max: nat)
   (#k: parser_kind)
   (#t: Type0)
-  (#p: parser k t)
+  (#err: Type0)
+  (#p: parser k t err)
   (s: serializer p)
   (elem_count_min: nat)
   (elem_count_max: nat)
@@ -335,11 +362,11 @@ let vlarray_to_vldata
     vldata_vlarray_precond array_byte_size_min array_byte_size_max p elem_count_min elem_count_max == true  
   })
   (x: vlarray t elem_count_min elem_count_max)
-: Tot (parse_bounded_vldata_strong_t array_byte_size_min array_byte_size_max (serialize_list _ s))
+: Tot (parse_bounded_vldata_strong_t array_byte_size_min array_byte_size_max (serialize_list _ () s))
 = [@inline_let]
   let x' : list t = x in
   [@inline_let]
-  let _ = vlarray_to_vldata_correct array_byte_size_min array_byte_size_max s elem_count_min elem_count_max x' in
+  let _ = vlarray_to_vldata_correct array_byte_size_min array_byte_size_max s elem_count_min elem_count_max x' () () in
   x'
 
 let vlarray_to_vldata_to_vlarray
@@ -347,7 +374,8 @@ let vlarray_to_vldata_to_vlarray
   (array_byte_size_max: nat)
   (#k: parser_kind)
   (#t: Type0)
-  (#p: parser k t)
+  (#err: Type0)
+  (#p: parser k t err)
   (s: serializer p)
   (elem_count_min: nat)
   (elem_count_max: nat)
@@ -366,19 +394,21 @@ let serialize_vlarray
   (array_byte_size_max: nat)
   (#k: parser_kind)
   (#t: Type0)
-  (#p: parser k t)
+  (#err: Type0)
+  (#p: parser k t err)
   (s: serializer p)
   (elem_count_min: nat)
   (elem_count_max: nat)
   (u: unit {
     vldata_vlarray_precond array_byte_size_min array_byte_size_max p elem_count_min elem_count_max == true  
   })
-: Tot (serializer (parse_vlarray array_byte_size_min array_byte_size_max s elem_count_min elem_count_max u))
+  (e_size_incomplete e_size_invalid e_payload: err)
+: Tot (serializer (parse_vlarray array_byte_size_min array_byte_size_max s elem_count_min elem_count_max u e_size_incomplete e_size_invalid e_payload))
 = vldata_to_vlarray_inj array_byte_size_min array_byte_size_max s elem_count_min elem_count_max u;
   vlarray_to_vldata_to_vlarray array_byte_size_min array_byte_size_max s elem_count_min elem_count_max u;
   serialize_synth
     _
     (vldata_to_vlarray array_byte_size_min array_byte_size_max s elem_count_min elem_count_max u)
-    (serialize_bounded_vldata_strong array_byte_size_min array_byte_size_max (serialize_list _ s))
+    (serialize_bounded_vldata_strong array_byte_size_min array_byte_size_max (serialize_list _ () s) e_size_incomplete e_size_invalid e_payload)
     (vlarray_to_vldata array_byte_size_min array_byte_size_max s elem_count_min elem_count_max u)
     ()
