src/lowparse/LowParse.Spec.FLData.fst
@@ -9,40 +9,45 @@ module Classical = FStar.Classical
 inline_for_extraction
 val parse_fldata'
   (#t: Type0)
-  (p: bare_parser t)
+  (#err: Type0)
+  (p: bare_parser t err)
   (sz: nat)
-: Tot (bare_parser t)
+  (e: err)
+: Tot (bare_parser t err)
 
-let parse_fldata' #t p sz =
+let parse_fldata' #t #err p sz e =
   let () = () in // Necessary to pass arity checking
   fun (s: bytes) ->
   if Seq.length s < sz
-  then None
+  then Error e
   else
     match p (Seq.slice s 0 sz) with
-    | Some (v, consumed) ->
+    | Correct (v, consumed) ->
       if (consumed <: nat) = (sz <: nat)
-      then Some (v, (sz <: consumed_length s))
-      else None
-    | _ -> None
+      then Correct (v, (sz <: consumed_length s))
+      else Error e
+    | Error e' -> Error e'
 
 let parse_fldata_injective
   (#k: parser_kind)
   (#t: Type0)
-  (p: parser k t)
+  (#err: Type0)
+  (p: parser k t err)
   (sz: nat)
+  (e: err)
 : Lemma
-  (ensures (injective (parse_fldata' p sz)))
+  (ensures (injective (parse_fldata' p sz e)))
 = let f
     (b1 b2: bytes)
   : Lemma
-    (requires (injective_precond (parse_fldata' p sz) b1 b2))
-    (ensures (injective_postcond (parse_fldata' p sz) b1 b2))
+    (requires (injective_precond (parse_fldata' p sz e) b1 b2))
+    (ensures (injective_postcond (parse_fldata' p sz e) b1 b2))
   = assert (injective_precond p (Seq.slice b1 0 sz) (Seq.slice b2 0 sz))
   in
   Classical.forall_intro_2 (fun b -> Classical.move_requires (f b))
 
 // unfold
+inline_for_extraction
 let parse_fldata_kind
   (sz: nat)
 : Tot parser_kind
@@ -54,47 +59,54 @@ inline_for_extraction
 val parse_fldata
   (#k: parser_kind)
   (#t: Type0)
-  (p: parser k t)
+  (#err: Type0)
+  (p: parser k t err)
   (sz: nat)
-: Tot (parser (parse_fldata_kind sz) t)
+  (e: err)
+: Tot (parser (parse_fldata_kind sz) t err)
 
-let parse_fldata #b #t p sz =
-  parse_fldata_injective p sz;
-  parse_fldata' p sz  
+let parse_fldata #b #t #err p sz e =
+  parse_fldata_injective p sz e;
+  parse_fldata' p sz e
 
 val parse_fldata_consumes_all
   (#t: Type0)
-  (p: bare_parser t)
+  (#err: Type0)
+  (p: bare_parser t err)
   (sz: nat)
-: Pure (bare_parser t)
+  (e: err)
+: Pure (bare_parser t err)
   (requires (consumes_all p))
   (ensures (fun _ -> True))
 
-let parse_fldata_consumes_all #t p sz =
+let parse_fldata_consumes_all #t #err p sz e =
   let () = () in // Necessary to pass arity checking
   fun (s: bytes) ->
   if Seq.length s < sz
-  then None
+  then Error e
   else
     match p (Seq.slice s 0 sz) with
-    | Some (v, _) ->
-      Some (v, (sz <: consumed_length s))
-    | _ -> None
+    | Correct (v, _) ->
+      Correct (v, (sz <: consumed_length s))
+    | Error e' -> Error e'
 
 let parse_fldata_consumes_all_correct
   (#k: parser_kind)
   (#t: Type0)
-  (p: parser k t)
+  (#err: Type0)
+  (p: parser k t err)
   (sz: nat)
+  (e: err)
 : Lemma
   (requires (k.parser_kind_subkind == Some ParserConsumesAll))
-  (ensures (forall b . parse (parse_fldata p sz) b == parse (parse_fldata_consumes_all p sz) b))
+  (ensures (forall b . parse (parse_fldata p sz e) b == parse (parse_fldata_consumes_all p sz e) b))
 = ()
 
 let parse_fldata_strong_pred
   (#k: parser_kind)
   (#t: Type0)
-  (#p: parser k t)
+  (#err: Type0)
+  (#p: parser k t err)
   (s: serializer p)
   (sz: nat)
   (x: t)
@@ -104,7 +116,8 @@ let parse_fldata_strong_pred
 let parse_fldata_strong_t
   (#k: parser_kind)
   (#t: Type0)
-  (#p: parser k t)
+  (#err: Type0)
+  (#p: parser k t err)
   (s: serializer p)
   (sz: nat)
 : Tot Type0
@@ -113,14 +126,16 @@ let parse_fldata_strong_t
 let parse_fldata_strong_correct
   (#k: parser_kind)
   (#t: Type0)
-  (#p: parser k t)
+  (#err: Type0)
+  (#p: parser k t err)
   (s: serializer p)
   (sz: nat)
+  (e: err)
   (xbytes: bytes)
   (consumed: consumed_length xbytes)
   (x: t)
 : Lemma
-  (requires (parse (parse_fldata p sz) xbytes == Some (x, consumed)))
+  (requires (parse (parse_fldata p sz e) xbytes == Correct (x, consumed)))
   (ensures (parse_fldata_strong_pred s sz x))
 = serializer_correct_implies_complete p s
 
@@ -128,20 +143,23 @@ inline_for_extraction
 let parse_fldata_strong
   (#k: parser_kind)
   (#t: Type0)
-  (#p: parser k t)
+  (#err: Type0)
+  (#p: parser k t err)
   (s: serializer p)
   (sz: nat)
-: Tot (parser (parse_fldata_kind sz) (parse_fldata_strong_t s sz))
+  (e: err)
+: Tot (parser (parse_fldata_kind sz) (parse_fldata_strong_t s sz) err)
 = coerce_parser
   (parse_fldata_strong_t s sz)
-  (parse_strengthen (parse_fldata p sz) (parse_fldata_strong_pred s sz) (parse_fldata_strong_correct s sz))
+  (parse_strengthen (parse_fldata p sz e) (parse_fldata_strong_pred s sz) (parse_fldata_strong_correct s sz e))
 
 #set-options "--z3rlimit 16"
 
 let serialize_fldata_strong'
   (#k: parser_kind)
   (#t: Type0)
-  (#p: parser k t)
+  (#err: Type0)
+  (#p: parser k t err)
   (s: serializer p)
   (sz: nat)
 : Tot (bare_serializer (parse_fldata_strong_t s sz))
@@ -151,8 +169,10 @@ let serialize_fldata_strong'
 let serialize_fldata_strong
   (#k: parser_kind)
   (#t: Type0)
-  (#p: parser k t)
+  (#err: Type0)
+  (#p: parser k t err)
   (s: serializer p)
   (sz: nat)
-: Tot (serializer (parse_fldata_strong s sz))
+  (e: err)
+: Tot (serializer (parse_fldata_strong s sz e))
 = serialize_fldata_strong' s sz
