src/lowparse/LowParse.Spec.Int.Aux.fst
@@ -18,23 +18,25 @@ let decode_u8_injective () : Lemma
   (make_total_constant_size_parser_precond 1 U8.t decode_u8)
 = ()
 
-let parse_u8: parser parse_u8_kind U8.t =
+let parse_u8 (#err: Type0) (e: err): parser parse_u8_kind U8.t err =
   decode_u8_injective ();
-  make_total_constant_size_parser 1 U8.t decode_u8
+  make_total_constant_size_parser 1 U8.t _ decode_u8 e
 
 let parse_u8_spec
+  (#err: Type0)
+  (e: err)
   (b: bytes)
 : Lemma
   (requires (Seq.length b >= 1))
   (ensures (
-    let pp = parse parse_u8 b in
-    Some? pp /\ (
-    let (Some (v, consumed)) = pp in
+    let pp = parse (parse_u8 e) b in
+    Correct? pp /\ (
+    let (Correct (v, consumed)) = pp in
     U8.v v == E.be_to_n (Seq.slice b 0 1)
   )))
 = ()
 
-let serialize_u8 : serializer parse_u8 =
+let serialize_u8 (#err: Type0) (e: err) : serializer (parse_u8 e) =
   Seq.create 1
 
 let decode_u16
@@ -70,26 +72,28 @@ let parse_u16_kind : parser_kind =
 
 #set-options "--z3rlimit 16"
 
-let parse_u16: parser parse_u16_kind U16.t =
+let parse_u16 (#err: Type0) (e: err): parser parse_u16_kind U16.t err =
   decode_u16_injective ();
   let p =
-    make_total_constant_size_parser 2 U16.t decode_u16
+    make_total_constant_size_parser 2 U16.t _ decode_u16 e
   in
   p
 
 let parse_u16_spec
+  (#err: Type0)
+  (e: err)
   (b: bytes)
 : Lemma
   (requires (Seq.length b >= 2))
   (ensures (
-    let pp = parse parse_u16 b in
-    Some? pp /\ (
-    let (Some (v, consumed)) = pp in
+    let pp = parse (parse_u16 e) b in
+    Correct? pp /\ (
+    let (Correct (v, consumed)) = pp in
     U16.v v == E.be_to_n (Seq.slice b 0 2)
   )))
-= let pp = parse parse_u16 b in
-  assert (Some? pp);
-  let (Some (v, _)) = pp in
+= let pp = parse (parse_u16 e) b in
+  assert (Correct? pp);
+  let (Correct (v, _)) = pp in
   let s = Seq.slice b 0 2 in
   assert (v == decode_u16 s);
   E.lemma_be_to_n_is_bounded s;
@@ -97,8 +101,11 @@ let parse_u16_spec
 
 #set-options "--z3rlimit 64"
 
-let serialize_u16 : serializer parse_u16 =
+let serialize_u16' : bare_serializer U16.t =
   (fun (x: U16.t) -> E.n_to_be 2ul (U16.v x))
+
+let serialize_u16 (#err: Type0) (e: err) : serializer (parse_u16 e) =
+  serialize_u16'
 
 #reset-options
 
@@ -134,25 +141,27 @@ let decode_u32_injective () : Lemma
 let parse_u32_kind : parser_kind =
   total_constant_size_parser_kind 4
 
-let parse_u32: parser parse_u32_kind U32.t =
+let parse_u32 (#err: Type0) (e: err): parser parse_u32_kind U32.t err =
   decode_u32_injective ();
-  make_total_constant_size_parser 4 U32.t decode_u32
+  make_total_constant_size_parser 4 U32.t _ decode_u32 e
 
 #set-options "--z3rlimit 16"
 
 let parse_u32_spec
+  (#err: Type0)
+  (e: err)
   (b: bytes)
 : Lemma
   (requires (Seq.length b >= 4))
   (ensures (
-    let pp = parse parse_u32 b in
-    Some? pp /\ (
-    let (Some (v, consumed)) = pp in
+    let pp = parse (parse_u32 e) b in
+    Correct? pp /\ (
+    let (Correct (v, consumed)) = pp in
     U32.v v == E.be_to_n (Seq.slice b 0 4)
   )))
-= let pp = parse parse_u32 b in
-  assert (Some? pp);
-  let (Some (v, _)) = pp in
+= let pp = parse (parse_u32 e) b in
+  assert (Correct? pp);
+  let (Correct (v, _)) = pp in
   let s = Seq.slice b 0 4 in
   assert (v == decode_u32 s);
   E.lemma_be_to_n_is_bounded s;
@@ -160,7 +169,10 @@ let parse_u32_spec
 
 #set-options "--z3rlimit 128"
 
-let serialize_u32 : serializer parse_u32 =
+let serialize_u32' : bare_serializer U32.t =
   (fun (x: U32.t) -> E.n_to_be 4ul (U32.v x))
+
+let serialize_u32 (#err: Type0) (e: err) : serializer (parse_u32 e) =
+  serialize_u32'
 
 #reset-options
