src/lowparse/LowParse.Spec.Int.fst
@@ -9,18 +9,24 @@ module U32 = FStar.UInt32
 
 let parse_u8 = Aux.parse_u8
 
-let parse_u8_spec b = Aux.parse_u8_spec b
+let parse_u8_spec = Aux.parse_u8_spec
+
+let parse_u8_spec_error #err e b = ()
 
 let serialize_u8 = Aux.serialize_u8
 
 let parse_u16 = Aux.parse_u16
 
-let parse_u16_spec b = Aux.parse_u16_spec b
+let parse_u16_spec = Aux.parse_u16_spec
+
+let parse_u16_spec_error #err e b = ()
 
 let serialize_u16 = Aux.serialize_u16
 
 let parse_u32 = Aux.parse_u32
 
 let parse_u32_spec = Aux.parse_u32_spec
+
+let parse_u32_spec_error #err e b = ()
 
 let serialize_u32 = Aux.serialize_u32
