src/lowparse/LowParse.Spec.Int.fsti
@@ -9,54 +9,93 @@ module U32 = FStar.UInt32
 
 let parse_u8_kind : parser_kind = total_constant_size_parser_kind 1
 
-val parse_u8: parser parse_u8_kind U8.t
+val parse_u8 (#err: Type0) (e: err): parser parse_u8_kind U8.t err
 
 val parse_u8_spec
+  (#err: Type0)
+  (e: err)
   (b: bytes)
 : Lemma
   (requires (Seq.length b >= 1))
   (ensures (
-    let pp = parse parse_u8 b in
-    Some? pp /\ (
-    let (Some (v, consumed)) = pp in
+    let pp = parse (parse_u8 e) b in
+    Correct? pp /\ (
+    let (Correct (v, consumed)) = pp in
     U8.v v == E.be_to_n (Seq.slice b 0 1)
   )))
 
-val serialize_u8 : serializer parse_u8
+val parse_u8_spec_error
+  (#err: Type0)
+  (e: err)
+  (b: bytes)
+: Lemma
+  (requires (Seq.length b < 1))
+  (ensures (
+    let pp = parse (parse_u8 e) b in
+    pp == Error e
+  ))
+
+val serialize_u8 (#err: Type0) (e: err) : serializer (parse_u8 e)
 
 inline_for_extraction
 let parse_u16_kind : parser_kind =
   total_constant_size_parser_kind 2
 
-val parse_u16: parser parse_u16_kind U16.t
+val parse_u16 (#err: Type0) (e: err): parser parse_u16_kind U16.t err
 
 val parse_u16_spec
+  (#err: Type0)
+  (e: err)
   (b: bytes)
 : Lemma
   (requires (Seq.length b >= 2))
   (ensures (
-    let pp = parse parse_u16 b in
-    Some? pp /\ (
-    let (Some (v, consumed)) = pp in
+    let pp = parse (parse_u16 e) b in
+    Correct? pp /\ (
+    let (Correct (v, consumed)) = pp in
     U16.v v == E.be_to_n (Seq.slice b 0 2)
   )))
 
-val serialize_u16 : serializer parse_u16
+val parse_u16_spec_error
+  (#err: Type0)
+  (e: err)
+  (b: bytes)
+: Lemma
+  (requires (Seq.length b < 2))
+  (ensures (
+    let pp = parse (parse_u16 e) b in
+    pp == Error e
+  ))
+
+val serialize_u16 (#err: Type0) (e: err) : serializer (parse_u16 e)
 
 let parse_u32_kind : parser_kind =
   total_constant_size_parser_kind 4
 
-val parse_u32: parser parse_u32_kind U32.t
+val parse_u32 (#err: Type0) (e: err): parser parse_u32_kind U32.t err
 
 val parse_u32_spec
+  (#err: Type0)
+  (e: err)
   (b: bytes)
 : Lemma
   (requires (Seq.length b >= 4))
   (ensures (
-    let pp = parse parse_u32 b in
-    Some? pp /\ (
-    let (Some (v, consumed)) = pp in
+    let pp = parse (parse_u32 e) b in
+    Correct? pp /\ (
+    let (Correct (v, consumed)) = pp in
     U32.v v == E.be_to_n (Seq.slice b 0 4)
   )))
 
-val serialize_u32 : serializer parse_u32
+val parse_u32_spec_error
+  (#err: Type0)
+  (e: err)
+  (b: bytes)
+: Lemma
+  (requires (Seq.length b < 4))
+  (ensures (
+    let pp = parse (parse_u32 e) b in
+    pp == Error e
+  ))
+
+val serialize_u32 (#err: Type0) (e: err) : serializer (parse_u32 e)
