src/lowparse/LowParse.Spec.List.fst
@@ -9,70 +9,83 @@ module Classical = FStar.Classical
 (* Parse a list, until there is nothing left to read. This parser will mostly fail EXCEPT if the whole size is known and the slice has been suitably truncated beforehand, or if the elements of the list all have a known constant size. *)
 
 val parse_list_aux
+  (#k: parser_kind)
   (#t: Type0)
-  (p: bare_parser t)
+  (#err: Type0)
+  (p: parser k t err)
+  (_: unit { k.parser_kind_low > 0 } )
   (b: bytes)
-: GTot (option (list t * (consumed_length b)))
+: GTot (result (list t * (consumed_length b)) err)
   (decreases (Seq.length b))
 
-let rec parse_list_aux #t p b =
+let rec parse_list_aux #k #t #err p u b =
   if Seq.length b = 0
   then 
-    Some ([], (0 <: consumed_length b))
+    Correct ([], (0 <: consumed_length b))
   else
     match p b with
-    | None -> None
-    | Some (v, n) ->
-      if n = 0
-      then None (* elements cannot be empty *)
-      else
-        match parse_list_aux p (Seq.slice b n (Seq.length b)) with
-	| Some (l, n') -> Some (v :: l, (n + n' <: consumed_length b))
-	| _ -> None
+    | Error e -> Error e
+    | Correct (v, n) ->
+      begin
+        match parse_list_aux p u (Seq.slice b n (Seq.length b)) with
+	| Correct (l, n') -> Correct (v :: l, (n + n' <: consumed_length b))
+	| Error e -> Error e
+      end
 
 val parse_list_bare
+  (#k: parser_kind)
   (#t: Type0)
-  (p: bare_parser t)
-: Tot (bare_parser (list t))
+  (#err: Type0)
+  (p: parser k t err)
+  (_: unit { k.parser_kind_low > 0 } )
+: Tot (bare_parser (list t) err)
 
-let parse_list_bare #t p = (fun b -> parse_list_aux #t p b) <: bare_parser (list t)
+let parse_list_bare #k #t #err p u = (fun b -> parse_list_aux #k #t #err p u b) <: bare_parser (list t) err
 
 let rec parse_list_bare_consumed
+  (#k: parser_kind)
   (#t: Type0)
-  (p: bare_parser t)
+  (#err: Type0)
+  (p: parser k t err)
+  (u: unit { k.parser_kind_low > 0 } )
   (b: bytes)
 : Lemma
-  (requires (Some? (parse_list_bare p b)))
+  (requires (Correct? (parse_list_bare p u b)))
   (ensures (
-    let pb = parse_list_bare p b in (
-    Some? pb /\ (
-    let (Some (_, consumed)) = pb in
+    let pb = parse_list_bare p u b in (
+    Correct? pb /\ (
+    let (Correct (_, consumed)) = pb in
     consumed == Seq.length b
   ))))
   (decreases (Seq.length b))
 = if Seq.length b = 0
   then ()
   else
-    let (Some (_, consumed1)) = p b in
+    let (Correct (_, consumed1)) = p b in
     let b' = Seq.slice b consumed1 (Seq.length b) in
-    parse_list_bare_consumed p b'
+    parse_list_bare_consumed p u b'
 
 let parse_list_bare_consumes_all
   (#k: parser_kind)
   (#t: Type0)
-  (p: parser k t)
+  (#err: Type0)
+  (p: parser k t err)
+  (u: unit { k.parser_kind_low > 0 } )
 : Lemma
-  (consumes_all (parse_list_bare p))
-= Classical.forall_intro (Classical.move_requires (parse_list_bare_consumed p))
+  (consumes_all (parse_list_bare p u))
+= Classical.forall_intro (Classical.move_requires (parse_list_bare_consumed p u))
 
 let no_lookahead_weak_on_parse_list_bare
+  (#k: parser_kind)
   (#t: Type0)
-  (p: bare_parser t)
+  (#err: Type0)
+  (p: parser k t err)
+  (u: unit { k.parser_kind_low > 0 } )
   (x x' : bytes)
 : Lemma
-  (no_lookahead_weak_on (parse_list_bare p) x x')
-= match parse_list_bare p x with
-  | Some _ -> parse_list_bare_consumed p x
+  (no_lookahead_weak_on (parse_list_bare p u) x x')
+= match parse_list_bare p u x with
+  | Correct _ -> parse_list_bare_consumed p u x
   | _ -> ()
 
 #set-options "--z3rlimit 16"
@@ -80,9 +93,11 @@ let no_lookahead_weak_on_parse_list_bare
 let parse_list_bare_injective
   (#k: parser_kind)
   (#t: Type0)
-  (p: parser k t)
+  (#err: Type0)
+  (p: parser k t err)
+  (u: unit { k.parser_kind_low > 0 } )
 : Lemma
-  (ensures (injective (parse_list_bare p)))
+  (ensures (injective (parse_list_bare p u)))
 = let f () : Lemma
     (injective p)
   = ()
@@ -91,8 +106,8 @@ let parse_list_bare_injective
     (b1: bytes)
     (b2: bytes)
   : Lemma
-    (requires (injective_precond (parse_list_bare p) b1 b2))
-    (ensures (injective_postcond (parse_list_bare p) b1 b2))
+    (requires (injective_precond (parse_list_bare p u) b1 b2))
+    (ensures (injective_postcond (parse_list_bare p u) b1 b2))
     (decreases (Seq.length b1 + Seq.length b2))
   = if Seq.length b1 = 0
     then begin
@@ -101,23 +116,24 @@ let parse_list_bare_injective
       assert (injective_precond p b1 b2);
       f ();
       assert (injective_postcond p b1 b2);
-      let (Some (_, len1)) = parse p b1 in
-      let (Some (_, len2)) = parse p b2 in
+      let (Correct (_, len1)) = parse p b1 in
+      let (Correct (_, len2)) = parse p b2 in
       assert ((len1 <: nat) == (len2 <: nat));
       let b1' : bytes = Seq.slice b1 len1 (Seq.length b1) in
       let b2' : bytes = Seq.slice b2 len2 (Seq.length b2) in
       aux b1' b2';
-      let (Some (_, len1')) = parse (parse_list_bare p) b1' in
-      let (Some (_, len2')) = parse (parse_list_bare p) b2' in
+      let (Correct (_, len1')) = parse (parse_list_bare p u) b1' in
+      let (Correct (_, len2')) = parse (parse_list_bare p u) b2' in
       Seq.lemma_split (Seq.slice b1 0 (len1 + len1')) len1;
       Seq.lemma_split (Seq.slice b2 0 (len2 + len2')) len2;
-      assert (injective_postcond (parse_list_bare p) b1 b2)
+      assert (injective_postcond (parse_list_bare p u) b1 b2)
     end
   in
   Classical.forall_intro_2 (fun b -> Classical.move_requires (aux b))
 
 #reset-options
 
+inline_for_extraction
 let parse_list_kind =
   {
     parser_kind_low = 0;
@@ -132,25 +148,29 @@ inline_for_extraction
 val parse_list
   (#k: parser_kind)
   (#t: Type0)
-  (p: parser k t)
-: Tot (parser parse_list_kind (list t))
+  (#err: Type0)
+  (p: parser k t err)
+  (u: unit { k.parser_kind_low > 0 } )
+: Tot (parser parse_list_kind (list t) err)
 
-let parse_list #k #t p =
-  Classical.forall_intro_2 (no_lookahead_weak_on_parse_list_bare p);
-  parse_list_bare_injective p;
-  parse_list_bare_consumes_all p;
-  parse_list_bare p
+let parse_list #k #t #err p u =
+  Classical.forall_intro_2 (no_lookahead_weak_on_parse_list_bare p u);
+  parse_list_bare_injective p u;
+  parse_list_bare_consumes_all p u;
+  parse_list_bare p u
 
 let rec bare_serialize_list
   (#k: parser_kind)
   (#t: Type0)
-  (p: parser k t)
+  (#err: Type0)
+  (p: parser k t err)
+  (u: unit { k.parser_kind_low > 0 } )
   (s: serializer p)
   (x: list t)
 : GTot bytes
 = match x with
   | [] -> Seq.createEmpty
-  | a :: q -> Seq.append (s a) (bare_serialize_list p s q)
+  | a :: q -> Seq.append (s a) (bare_serialize_list p u s q)
 
 unfold
 let serialize_list_precond
@@ -162,66 +182,74 @@ let serialize_list_precond
 let bare_serialize_list_correct
   (#k: parser_kind)
   (#t: Type0)
-  (p: parser k t)
+  (#err: Type0)
+  (p: parser k t err)
+  (u: unit { k.parser_kind_low > 0 } )
   (s: serializer p)
 : Lemma
   (requires (serialize_list_precond k))
-  (ensures (serializer_correct (parse_list p) (bare_serialize_list p s)))
+  (ensures (serializer_correct (parse_list p u) (bare_serialize_list p u s)))
 = let f () : Lemma (serialize_list_precond k) = () in
   let rec prf
     (l: list t)
   : Lemma
-    (parse (parse_list p) (bare_serialize_list p s l) == Some (l, Seq.length (bare_serialize_list p s l)))
+    (parse (parse_list p u) (bare_serialize_list p u s l) == Correct (l, Seq.length (bare_serialize_list p u s l)))
   = match l with
     | [] -> ()
     | a :: q ->
-      let pa = parse p (bare_serialize_list p s l) in
+      let pa = parse p (bare_serialize_list p u s l) in
       f ();
-      assert (no_lookahead_on p (s a) (bare_serialize_list p s l));
-      seq_slice_append_l (s a) (bare_serialize_list p s q);
-      assert (no_lookahead_on_precond p (s a) (bare_serialize_list p s l));
-      assert (no_lookahead_on_postcond p (s a) (bare_serialize_list p s l));
-      assert (Some? pa);
-      assert (injective_precond p (s a) (bare_serialize_list p s l));
-      assert (injective_postcond p (s a) (bare_serialize_list p s l));
-      let (Some (a', lena)) = pa in
+      assert (no_lookahead_on p (s a) (bare_serialize_list p u s l));
+      seq_slice_append_l (s a) (bare_serialize_list p u s q);
+      assert (no_lookahead_on_precond p (s a) (bare_serialize_list p u s l));
+      assert (no_lookahead_on_postcond p (s a) (bare_serialize_list p u s l));
+      assert (Correct? pa);
+      assert (injective_precond p (s a) (bare_serialize_list p u s l));
+      assert (injective_postcond p (s a) (bare_serialize_list p u s l));
+      let (Correct (a', lena)) = pa in
       assert (a == a');
       assert (lena == Seq.length (s a));
       assert (lena > 0);
       prf q;
-      seq_slice_append_r (s a) (bare_serialize_list p s q)
+      seq_slice_append_r (s a) (bare_serialize_list p u s q)
   in
   Classical.forall_intro prf
 
 let serialize_list
   (#k: parser_kind)
   (#t: Type0)
-  (p: parser k t)
+  (#err: Type0)
+  (p: parser k t err)
+  (u: unit { k.parser_kind_low > 0 } )
   (s: serializer p)
-: Pure (serializer (parse_list p))
+: Pure (serializer (parse_list p u))
   (requires (
     serialize_list_precond k
   ))
   (ensures (fun _ -> True))
-= bare_serialize_list_correct p s;
-  bare_serialize_list p s
+= bare_serialize_list_correct p u s;
+  bare_serialize_list p u s
 
 let serialize_list_nil
   (#k: parser_kind)
   (#t: Type0)
-  (p: parser k t)
+  (#err: Type0)
+  (p: parser k t err)
+  (u: unit { k.parser_kind_low > 0 } )
   (s: serializer p)
 : Lemma
   (requires (
     serialize_list_precond k
   ))
-  (ensures (serialize (serialize_list p s) [] == Seq.createEmpty))
+  (ensures (serialize (serialize_list p u s) [] == Seq.createEmpty))
 = ()
 
 let serialize_list_cons
   (#k: parser_kind)
   (#t: Type0)
-  (p: parser k t)
+  (#err: Type0)
+  (p: parser k t err)
+  (u: unit { k.parser_kind_low > 0 } )
   (s: serializer p)
   (a: t)
   (q: list t)
@@ -230,65 +258,71 @@ let serialize_list_cons
     serialize_list_precond k
   ))
   (ensures (
-    serialize (serialize_list p s) (a :: q) == Seq.append (serialize s a) (serialize (serialize_list p s) q)
+    serialize (serialize_list p u s) (a :: q) == Seq.append (serialize s a) (serialize (serialize_list p u s) q)
   ))
 = ()
 
 let serialize_list_singleton
   (#k: parser_kind)
   (#t: Type0)
-  (p: parser k t)
+  (#err: Type0)
+  (p: parser k t err)
+  (u: unit { k.parser_kind_low > 0 } )
   (s: serializer p)
   (a: t)
 : Lemma
   (requires (serialize_list_precond k))
-  (ensures (serialize (serialize_list p s) [a] == serialize s a))
+  (ensures (serialize (serialize_list p u s) [a] == serialize s a))
 = Seq.append_empty_r (serialize s a)
 
 let rec serialize_list_append
   (#k: parser_kind)
   (#t: Type0)
-  (p: parser k t)
+  (#err: Type0)
+  (p: parser k t err)
+  (u: unit { k.parser_kind_low > 0 } )
   (s: serializer p)
   (l1 l2: list t)
 : Lemma
   (requires (serialize_list_precond k))
-  (ensures (serialize (serialize_list p s) (L.append l1 l2) == Seq.append (serialize (serialize_list p s) l1) (serialize (serialize_list p s) l2)))
+  (ensures (serialize (serialize_list p u s) (L.append l1 l2) == Seq.append (serialize (serialize_list p u s) l1) (serialize (serialize_list p u s) l2)))
 = match l1 with
   | a :: q ->
-    serialize_list_append p s q l2;
-    Seq.append_assoc (serialize s a) (serialize (serialize_list p s) q) (serialize (serialize_list p s) l2)
+    serialize_list_append p u s q l2;
+    Seq.append_assoc (serialize s a) (serialize (serialize_list p u s) q) (serialize (serialize_list p u s) l2)
   | [] ->
-    Seq.append_empty_l (serialize (serialize_list p s) l2)
+    Seq.append_empty_l (serialize (serialize_list p u s) l2)
 
 val list_length_constant_size_parser_correct
   (#k: parser_kind)
   (#t: Type0)
-  (p: parser k t)
+  (#err: Type0)
+  (p: parser k t err)
+  (u: unit { k.parser_kind_low > 0 } )
   (b: bytes)
 : Lemma
   (requires (
     k.parser_kind_high == Some k.parser_kind_low /\
-    Some? (parse (parse_list p) b)
+    Correct? (parse (parse_list p u) b)
   ))
   (ensures (
-    let pb = parse (parse_list p) b in
-    Some? pb /\ (
-    let (Some (l, _)) = pb in
+    let pb = parse (parse_list p u) b in
+    Correct? pb /\ (
+    let (Correct (l, _)) = pb in
     FStar.Mul.op_Star (L.length l) k.parser_kind_low == Seq.length b
   )))
   (decreases (Seq.length b))
 
-let rec list_length_constant_size_parser_correct #k #t p b =
+let rec list_length_constant_size_parser_correct #k #t #err p u b =
   let n = k.parser_kind_low in
   if Seq.length b = 0
   then ()
   else begin
-    let (Some (_, consumed)) = parse p b in
+    let (Correct (_, consumed)) = parse p b in
     assert ((consumed <: nat) == n);
     assert (n > 0);
     let b' : bytes = Seq.slice b n (Seq.length b) in
-    list_length_constant_size_parser_correct p b';
-    let (Some (l', _)) = parse (parse_list p) b' in
+    list_length_constant_size_parser_correct p u b';
+    let (Correct (l', _)) = parse (parse_list p u) b' in
     FStar.Math.Lemmas.distributivity_add_left 1 (L.length l') n
   end
