src/lowparse/LowParse.Spec.Seq.fst
@@ -10,26 +10,28 @@ module Classical = FStar.Classical
 (* Parse a list, until there is nothing left to read. This parser will mostly fail EXCEPT if the whole size is known and the slice has been suitably truncated beforehand, or if the elements of the list all have a known constant size. *)
 
 val parse_seq_aux
+  (#k: parser_kind)
   (#t: Type0)
-  (p: bare_parser t)
+  (#err: Type0)
+  (p: parser k t err)
+  (u: unit { k.parser_kind_low > 0 } )
   (b: bytes)
-: GTot (option (Seq.seq t * (consumed_length b)))
+: GTot (result (Seq.seq t * (consumed_length b)) err)
   (decreases (Seq.length b))
 
-let rec parse_seq_aux #t p b =
+let rec parse_seq_aux #k #t #err p u b =
   if Seq.length b = 0
   then 
-    Some (Seq.createEmpty, (0 <: consumed_length b))
+    Correct (Seq.createEmpty, (0 <: consumed_length b))
   else
     match p b with
-    | None -> None
-    | Some (v, n) ->
-      if n = 0
-      then None (* elements cannot be empty *)
-      else
-        match parse_seq_aux p (Seq.slice b n (Seq.length b)) with
-	| Some (l, n') -> Some (Seq.cons v l, (n + n' <: consumed_length b))
-	| _ -> None
+    | Error e -> Error e
+    | Correct (v, n) ->
+      begin
+        match parse_seq_aux p u (Seq.slice b n (Seq.length b)) with
+	| Correct (l, n') -> Correct (Seq.cons v l, (n + n' <: consumed_length b))
+	| Error e -> Error e
+      end
 
 let seq_of_list_inj
   (t: Type0)
@@ -40,35 +42,36 @@ let seq_of_list_inj
 let parse_seq'
   (#k: parser_kind)
   (#t: Type0)
-  (p: parser k t)
-: Tot (parser PL.parse_list_kind (Seq.seq t))
+  (#err: Type0)
+  (p: parser k t err)
+  (u: unit { k.parser_kind_low > 0 } )
+: Tot (parser PL.parse_list_kind (Seq.seq t) err)
 = seq_of_list_inj t;
-  parse_synth (PL.parse_list p) (Seq.seq_of_list)
+  parse_synth (PL.parse_list p u) (Seq.seq_of_list)
 
 val parse_seq_aux_correct
   (#k: parser_kind)
   (#t: Type0)
-  (p: parser k t)
+  (#err: Type0)
+  (p: parser k t err)
+  (u: unit { k.parser_kind_low > 0 } )
   (b: bytes)
 : Lemma
   (ensures (
-    parse (parse_seq_aux p) b == parse (parse_seq' p) b
+    parse (parse_seq_aux p u) b == parse (parse_seq' p u) b
   ))
   (decreases (Seq.length b))
 
 #set-options "--z3rlimit 32"
 
-let rec parse_seq_aux_correct #k #t p b =
+let rec parse_seq_aux_correct #k #t #err p u b =
   if Seq.length b = 0
   then ()
   else
     match parse p b with
-    | Some (v, n) ->
-      if n = 0
-      then ()
-      else
+    | Correct (v, n) ->
 	let b' = Seq.slice b n (Seq.length b) in
-	parse_seq_aux_correct p b'
+	parse_seq_aux_correct p u b'
     | _ -> ()
 
 #reset-options
@@ -76,64 +79,74 @@ let rec parse_seq_aux_correct #k #t p b =
 let parse_seq
   (#k: parser_kind)
   (#t: Type0)
-  (p: parser k t)
-: Tot (parser PL.parse_list_kind (Seq.seq t))
-= Classical.forall_intro (parse_seq_aux_correct p);
-  no_lookahead_weak_ext (parse_seq' p) (parse_seq_aux p);
-  injective_ext (parse_seq' p) (parse_seq_aux p);
-  no_lookahead_ext (parse_seq' p) (parse_seq_aux p);
-  parse_seq_aux p
+  (#err: Type0)
+  (p: parser k t err)
+  (u: unit { k.parser_kind_low > 0 } )
+: Tot (parser PL.parse_list_kind (Seq.seq t) err)
+= Classical.forall_intro (parse_seq_aux_correct p u);
+  no_lookahead_weak_ext (parse_seq' p u) (parse_seq_aux p u);
+  injective_ext (parse_seq' p u) (parse_seq_aux p u);
+  no_lookahead_ext (parse_seq' p u) (parse_seq_aux p u);
+  parse_seq_aux p u
 
 let parse_seq_correct
   (#k: parser_kind)
   (#t: Type0)
-  (p: parser k t)
+  (#err: Type0)
+  (p: parser k t err)
+  (u: unit { k.parser_kind_low > 0 } )
   (b: bytes)
 : Lemma
-  (parse (parse_seq p) b == parse (parse_seq' p) b)
-= parse_seq_aux_correct p b
+  (parse (parse_seq p u) b == parse (parse_seq' p u) b)
+= parse_seq_aux_correct p u b
 
 val seq_length_constant_size_parser_correct
   (#k: parser_kind)
   (#t: Type0)
-  (p: parser k t)
+  (#err: Type0)
+  (p: parser k t err)
+  (u: unit { k.parser_kind_low > 0 } )
   (b: bytes)
 : Lemma
   (requires (
     k.parser_kind_high == Some k.parser_kind_low /\
-    Some? (parse (parse_seq p) b)
+    Correct? (parse (parse_seq p u) b)
   ))
   (ensures (
-    let pb = parse (parse_seq p) b in
-    Some? pb /\ (
-    let (Some (l, _)) = pb in
+    let pb = parse (parse_seq p u) b in
+    Correct? pb /\ (
+    let (Correct (l, _)) = pb in
     FStar.Mul.op_Star (Seq.length l) k.parser_kind_low == Seq.length b
   )))
 
-let seq_length_constant_size_parser_correct #k #t p b =
-  parse_seq_correct p b;
-  PL.list_length_constant_size_parser_correct p b
+let seq_length_constant_size_parser_correct #k #t #err p u b =
+  parse_seq_correct p u b;
+  PL.list_length_constant_size_parser_correct p u b
 
 let serialize_seq'
   (#k: parser_kind)
   (#t: Type0)
-  (p: parser k t)
+  (#err: Type0)
+  (p: parser k t err)
+  (u: unit { k.parser_kind_low > 0 } )
   (s: serializer p)
-: Pure (serializer (parse_seq' p))
+: Pure (serializer (parse_seq' p u))
   (requires (PL.serialize_list_precond k))
   (ensures (fun _ -> True))
 = Classical.forall_intro (Seq.lemma_seq_list_bij #t);
   Classical.forall_intro (Seq.lemma_list_seq_bij #t);
-  serialize_synth (PL.parse_list p) Seq.seq_of_list (PL.serialize_list p s) Seq.seq_to_list ()
+  serialize_synth (PL.parse_list p u) Seq.seq_of_list (PL.serialize_list p u s) Seq.seq_to_list ()
 
 let serialize_seq
   (#k: parser_kind)
   (#t: Type0)
-  (p: parser k t)
+  (#err: Type0)
+  (p: parser k t err)
+  (u: unit { k.parser_kind_low > 0 } )
   (s: serializer p)
-: Pure (serializer (parse_seq p))
+: Pure (serializer (parse_seq p u))
   (requires (PL.serialize_list_precond k))
   (ensures (fun _ -> True))
-= Classical.forall_intro (parse_seq_correct p);
-  serialize_ext (parse_seq' p) (serialize_seq' p s) (parse_seq p)
+= Classical.forall_intro (parse_seq_correct p u);
+  serialize_ext (parse_seq' p u) (serialize_seq' p u s) (parse_seq p u)
 
